Implement tcc_no_lift, which tries to return the non-lifted effect of a term
When inspecting the effect of terms, tcc returns the potentially lifted
effects, which is not what we want because the original effectful information is
then cluttered. In the worst case, F* gives the effect information in terms of a
quite primitive effect, like STATE, which can't be easily exploited by
the user. Besides, it also causes problem for the functions which
explore the context to find suitable state variables with which to
instantiate pre/postconditions.
As this is mostly a problem for applications, the current workaround is,
in case of applications, to strip the parameters, retrieve the head's
effect with tcc, and instantiate this effect. In the other situations we
just use tcc.
Note that we tried inspecting then repacking the term just before the
call to tcc to check if it allows to "forget" about the context, but it
doesn't work.

FEM.Process.fst
@@ -579,6 +579,29 @@ let rec unfold_until_arrow e ty =
     (* Other situations: don't know what to do *)
     mfail ("unfold_until_arrow: could not unfold: " ^ term_to_string ty)
 
+/// Instantiate a comp
+val inst_comp_once : env -> comp -> term -> Tac comp
+let inst_comp_once e c t =
+  let ty = get_comp_ret_type c in
+  let ty' = unfold_until_arrow e ty in
+  begin match inspect ty' with
+  | Tv_Arrow b1 c1 ->
+    subst_binder_in_comp e b1 t c1
+  | _ -> (* Inconsistent state *)
+    mfail "inst_comp_once: inconsistent state"
+  end
+
+val inst_comp : env -> comp -> list term -> Tac comp
+let rec inst_comp e c tl =
+  match tl with
+  | [] -> c
+  | t :: tl' ->
+    let c' = try inst_comp_once e c t
+             with | MetaAnalysis msg -> mfail ("inst_comp: error: " ^ msg)
+                  | err -> raise err
+    in
+    inst_comp e c' tl'
+
 /// Update the current ``typ_or_comp`` before going into the body of an abstraction.
 /// Explanations:
 /// In the case we dive into a term of the form:
@@ -984,6 +1007,39 @@ let compute_effect_info dbg e tm =
   | Some c -> comp_to_effect_info dbg c
   | None -> None
 
+/// Converts a ``typ_or_comp`` to an ``effect_info`` by applying the instantiation
+/// stored in the ``typ_or_comp``.
+let typ_or_comp_to_effect_info (dbg : bool) (ge : genv) (c : typ_or_comp) :
+  Tac effect_info =
+  match c with
+  | TC_Typ ty _ ->
+    let tinfo = get_type_info_from_type ty in
+    mk_effect_info E_Total tinfo None None
+  | TC_Comp cv _ ->
+    let opt_einfo = comp_to_effect_info dbg cv in
+    match opt_einfo with
+    | None -> mfail ("typ_or_comp_to_effect_info failed on: " ^ acomp_to_string cv)
+    | Some einfo -> einfo
+
+/// `tcc` often returns a lifted effect which is not what we want (ex.: a
+/// lemma called inside a Stack function may have been lifted to Stack, but
+/// when studying this term effect, we want to retrieve its non-lifted effect).
+/// The workaround is to decompose the term if it is an application, then retrieve
+/// the effect of the head, and reconstruct it.
+/// Note: I tried inspecting then repacking the term before calling ``tcc`` to
+/// see if it allows to "forget" the context: it doesn't work.
+val tcc_no_lift : env -> term -> Tac comp
+
+let tcc_no_lift e t =
+  match inspect t with
+  | Tv_App _ _ ->
+    let hd, args = collect_app t in
+    let c = tcc e hd in
+    inst_comp e c (List.Tot.map fst args)
+  | _ ->
+    (* Fall back to ``tcc`` *)
+    tcc e t
+
 /// Returns the effectful information about a term
 val compute_eterm_info : dbg:bool -> env -> term -> Tac eterm_info
 
@@ -993,7 +1049,7 @@ let compute_eterm_info (dbg : bool) (e : env) (t : term) =
   let hd, parameters = decompose_application e t in
   try
     begin
-    let c : comp = tcc e t in
+    let c : comp = tcc_no_lift e t in
     let opt_einfo = comp_to_effect_info dbg c in
     match opt_einfo with
     | None -> mfail ("compute_eterm_info: failed on: " ^ term_to_string t)
@@ -1134,20 +1190,6 @@ let generate_shadowed_subst ge =
   let bl = List.Tot.map mk_binder bvl in
   let dummy = mk_abs (`()) bl in
   _generate_shadowed_subst ge dummy bvl
-
-/// Converts a ``typ_or_comp`` to an ``effect_info`` by applying the instantiation
-/// stored in the ``typ_or_comp``.
-let typ_or_comp_to_effect_info (dbg : bool) (ge : genv) (c : typ_or_comp) :
-  Tac effect_info =
-  match c with
-  | TC_Typ ty _ ->
-    let tinfo = get_type_info_from_type ty in
-    mk_effect_info E_Total tinfo None None
-  | TC_Comp cv _ ->
-    let opt_einfo = comp_to_effect_info dbg cv in
-    match opt_einfo with
-    | None -> mfail ("typ_or_comp_to_effect_info failed on: " ^ acomp_to_string cv)
-    | Some einfo -> einfo
 
 (*/// Retrieve the list of types from the parameters stored in ``typ_or_comp``.
 val typ_or_comp_to_param_types : typ_or_comp -> Tot (list typ)
@@ -2260,6 +2302,7 @@ let analyze_effectful_term dbg with_gpre with_gpost res =
     | _ -> (ge, res.res, compute_eterm_info dbg ge.env res.res, None, None, false)
     end
   in
+  print_dbg dbg ("[> Focused term constructor: " ^ term_construct studied_term);
   print_dbg dbg ("[> Environment information (after effect analysis):\n" ^ genv_to_string ge1);
   (* Check if the considered term is an assert, in which case we will only
    * display the precondition (otherwise we introduce too many assertions
